Langlib/Languages/Subleq.lean
@@ -1,6 +1,7 @@
 import Langlib.Languages.Subleq.Syntax
 import Langlib.Languages.Subleq.Parser
 import Langlib.Languages.Subleq.Semantics
+import Langlib.Languages.Subleq.Trace
 
 /-!
 # Subleq
