Langlib/Tests/Main.lean
@@ -27,6 +27,7 @@ import Langlib.Tests.Piet
 import Langlib.Tests.Ski
 import Langlib.Tests.Subleq
 import Langlib.Tests.URMFractran
+import Langlib.Tests.SubleqTrace
 import Langlib.Tests.TurpentineTrace
 import Langlib.Tests.WhitespaceTrace
 import Langlib.Tests.URMBrainfuck
@@ -79,6 +80,7 @@ def main : IO UInt32 :=
     , Langlib.Tests.Piet.suites
     , Langlib.Tests.Ski.suites
     , Langlib.Tests.Subleq.suites
+    , Langlib.Tests.SubleqTrace.suites
     , Langlib.Tests.TurpentineTrace.suites
     , Langlib.Tests.WhitespaceTrace.suites
     , Langlib.Tests.URMBrainfuck.suites
